Proofs for other store operations

SP1Chips/StoreDoubleChip.lean
@@ -1,5 +1,5 @@
 import SP1Foundations
-import SP1Chips.Store.StoreByte.Constraints
+import SP1Chips.Store.StoreDouble.Constraints
 import SP1Operations.Operation.AddrAddOperation
 
 open LeanRV64D.Functions Sail SailState
@@ -18,40 +18,48 @@ namespace Store
 
 noncomputable def spec_sb (imm : BitVec 12) (rs1 rs2 : regidx) : SailM ExecutionResult := do
   Sail.writeReg Register.nextPC ((← Sail.readReg Register.PC) + 4#64)
-  let width : ℕ := 1 -- single byte
+  let width : ℕ := 8 -- eight bytes
   execute_STORE imm rs1 rs2 width
 
-def sp1_op_a (Main : Vector (Fin BB) 50) : BitVec 5 :=
+def sp1_op_a (Main : Vector (Fin BB) 39) : BitVec 5 :=
   BitVec.ofNat 5 Main[6]
 
-def sp1_ob_b (Main : Vector (Fin BB) 50) : BitVec 5 :=
+def sp1_ob_b (Main : Vector (Fin BB) 39) : BitVec 5 :=
   BitVec.ofNat 5 Main[14]
 
-def sp1_imm_c (Main : Vector (Fin BB) 50) : BitVec 12 :=
+def sp1_imm_c (Main : Vector (Fin BB) 39) : BitVec 12 :=
   BitVec.ofNat 12 (Word.toNat #v[Main[21], Main[22], Main[23], Main[24]])
 
-def sp1_sb (Main : Vector (Fin BB) 50) : SailM ExecutionResult := do
+def sp1_sb (Main : Vector (Fin BB) 39) : SailM ExecutionResult := do
   let op_a := sp1_op_a Main
   Sail.writeReg Register.nextPC (Word.toBitVec64 #v[Main[3] + 4, Main[4], Main[5], 0])
   let addr : BitVec 64 := Word.toBitVec64 #v[Main[25], Main[26], Main[27], 0]
-  Sail.write_ram 64 1 0#64 addr (Word.toBitVec64 #v[Main[7], Main[8], Main[9], Main[10]])
+  Sail.write_ram 64 8 0#64 addr (Word.toBitVec64 #v[Main[7], Main[8], Main[9], Main[10]])
   return RETIRE_SUCCESS
 
-lemma run_vmem_write_of_width_1'
+lemma run_vmem_write_of_width_8
     (rs_addr_bv : BitVec 5)
     (reg_val : BitVec 64) -- thing inside `rs_addr_bv`
     (offset : BitVec 64)
-    (data : BitVec 8) -- bigger for others
+    (data : BitVec 64) -- bigger for others
     (s : SailState)
     (hs : SailState.isInitialized s)
     (h_reg_val : s.get_reg? rs_addr_bv = some reg_val)
-    (h_aligned : is_aligned_vaddr (virtaddr.Virtaddr (reg_val + offset)) 1 = true) ---width
+    (h_aligned : is_aligned_vaddr (virtaddr.Virtaddr (reg_val + offset)) 8 = true) ---width
     (hconfig : SailState.isValidMemConfig s hs)
-    (h_does_fit : reg_val.toNat + offset.toNat + 1 ≤ --width
+    (h_does_fit : reg_val.toNat + offset.toNat + 8 ≤ --width
       (s.regs.get Register.plat_ram_size (hs _)).toNat) :
-    (vmem_write (.Regidx rs_addr_bv) offset 1 data
+    (vmem_write (.Regidx rs_addr_bv) offset 8 data
       (AccessType.Write Data) false false false).run s = .ok (.Ok true)
-        { s with mem := s.mem.insert (reg_val + offset).toNat (BitVec.ofNat 8 data.toNat) } := by
+        { s with mem := ((((((((s.mem.insert
+          (reg_val + offset).toNat (BitVec.ofNat 8 data.toNat)).insert
+          ((reg_val + offset).toNat + 1) (BitVec.ofNat 8 (data.toNat >>> 8))).insert
+          ((reg_val + offset).toNat + 2) (BitVec.ofNat 8 (data.toNat >>> 16))).insert
+          ((reg_val + offset).toNat + 3) (BitVec.ofNat 8 (data.toNat >>> 24))).insert
+          ((reg_val + offset).toNat + 4) (BitVec.ofNat 8 (data.toNat >>> 32))).insert
+          ((reg_val + offset).toNat + 5) (BitVec.ofNat 8 (data.toNat >>> 40))).insert
+          ((reg_val + offset).toNat + 6) (BitVec.ofNat 8 (data.toNat >>> 48))).insert
+          ((reg_val + offset).toNat + 7) (BitVec.ofNat 8 (data.toNat >>> 56))) } := by
   obtain ⟨h_mprv_disabled, h_cur_privilege, h_clint_base, h_clint_size,
     h_plat_ram_base, h_plat_rom_base⟩ := hconfig
   have hmachine : (Privilege.Machine == Privilege.Machine) = true := rfl
@@ -68,25 +76,25 @@ lemma run_vmem_write_of_width_1'
   simp [effectivePrivilege, hfetch, h_mprv_disabled]
   simp [mem_write_value_priv_meta, checked_mem_write, h_cur_privilege, phys_access_check, SailME.run]
   simp [LeanRV64D.Functions.sys_pmp_count, pmp_check_machine reg_val offset s hs]
-  simp [run_within_mmio_writable_mmio reg_val offset s hs h_clint_base h_clint_size]
+  simp [run_within_mmio_writable_mmio reg_val offset 8 (by omega) s hs h_clint_base h_clint_size]
   simp [zero_extend, BitVec.addInt, Sail.BitVec.zeroExtend]
-  simp [run_within_phys_mem reg_val offset 1 s hs h_plat_ram_base h_plat_rom_base h_does_fit]
+  simp [run_within_phys_mem reg_val offset 8 s hs h_plat_ram_base h_plat_rom_base h_does_fit]
   simp [write_kind_of_flags, phys_mem_write, LeanRV64D.Functions.write_ram,
     sail_mem_write, PreSail.sail_mem_write, PreSail.writeBytes,
     PreSail.writeByte, Except.map, BitVec.addInt]
 
 set_option debug.skipKernelTC true in
-theorem correct (Main : Vector (Fin BB) 50)
+theorem correct (Main : Vector (Fin BB) 39)
     (s : SailState) (hs : SailState.isInitialized s)
     (hs_config : SailState.isValidMemConfig s hs)
-    (h_cstrs : (StoreByte.constraints Main).allHold)
-    (state_cstrs : (StoreByte.constraints Main).initialState s)
-    (h_is_real : Main[49] = 1)
+    (h_cstrs : (StoreDouble.constraints Main).allHold)
+    (state_cstrs : (StoreDouble.constraints Main).initialState s)
+    (h_is_real : Main[38] = 1)
     (h_fits_in_mem :
       let reg_val := (Word.toBitVec64 #v[Main[15], Main[16], Main[17], Main[18]]).toNat
       let offset := (BitVec.signExtend 64 (sp1_imm_c Main)).toNat
       let ram_size := (s.regs.get Register.plat_ram_size (hs _)).toNat
-      reg_val + offset + 1 ≤ ram_size) :
+      reg_val + offset + 8 ≤ ram_size) :
     let op_a := sp1_op_a Main
     let op_b := sp1_ob_b Main
     let imm_c := sp1_imm_c Main
@@ -98,26 +106,27 @@ theorem correct (Main : Vector (Fin BB) 50)
     h_plat_ram_base, h_plat_rom_base⟩ := hs_config
 
   -- Extract the main constraints from the chip
-  rw [StoreByte.constraints] at h_cstrs
+  rw [StoreDouble.constraints] at h_cstrs
   simp [SP1ConstraintList.allHold] at h_cstrs
   simp [AddressOperation.constraints, sub_eq_zero, h_is_real] at h_cstrs
-  obtain ⟨h_add_addr, h49, h38, h39, h40, h49, h_cpu, h_reader, h_cstrs⟩ := h_cstrs
+  obtain ⟨h_add_addr, h38, h39, h_cpu, h_reader, h_cstrs⟩ := h_cstrs
 
   -- Extract constraints about the state of operations
-  simp [StoreByte.constraints, AddressOperation.constraints,
+  simp [StoreDouble.constraints, AddressOperation.constraints,
     SP1Constraint.toStateProp, AddrAddOperation.constraints,
     CPUState.constraints, ITypeReaderImmutable.constraints,
-    Opcode.ofNat, Nat.ble, h_is_real] at state_cstrs
+    Opcode.ofNat, Nat.ble, h_is_real, Nat.beq] at state_cstrs
   obtain ⟨h_read_pc, h6_op_a, h14_op_a, h_imm_state⟩ := state_cstrs
   rw [Std.ExtDHashMap.get?_eq_some_get (hs _), Option.some_inj] at h_read_pc
 
   -- Extract constraints about the reader
   simp [ITypeReaderImmutable.constraints,
-      SP1Constraint.toProp, Opcode.ofNat, Nat.ble] at h_reader
+      SP1Constraint.toProp, Opcode.ofNat, Nat.ble, Nat.beq] at h_reader
   have h_imm_c : Word.toBitVec64 #v[Main[21], Main[22], Main[23], Main[24]] =
       BitVec.signExtend 64 (BitVec.ofNat 12 Main[21]) := by clear *- h_reader; simp_all only
   have h6_32 : Main[6] < 32 := by clear *- h_reader; simp_all only
   have h14_32 : Main[14] < 32 := by clear *- h_reader; simp_all only
+
   specialize h6_op_a h6_32
   specialize h14_op_a h14_32
   have h15u64 : Word.isU64 #v[Main[15], Main[16], Main[17], Main[18]] := by
@@ -140,13 +149,13 @@ theorem correct (Main : Vector (Fin BB) 50)
   simp [sp1_sb, haddr_add.2]
 
   -- Apply the main helper lemma
-  rw [run_vmem_write_of_width_1' (BitVec.ofNat 5 Main[14])
+  rw [run_vmem_write_of_width_8 (BitVec.ofNat 5 Main[14])
     (Word.toBitVec64 #v[Main[15], Main[16], Main[17], Main[18]])
     (BitVec.signExtend 64 imm_c)
     (Word.toBitVec64 #v[Main[7], Main[8], Main[9], Main[10]])]
 
   -- Arithmetic Caclulations
-  · simp [sp1_sb, h_imm_c, imm_c, Sail.write_ram, PreSail.write_ram,
+  · simp [sp1_sb, h_imm_c, imm_c, sp1_imm_c, Sail.write_ram, PreSail.write_ram,
       PreSail.writeBytes, PreSail.writeByte]
     constructor
     · simp [Word.toBitVec64, Word.toNat, Fin.val_add]
@@ -154,18 +163,15 @@ theorem correct (Main : Vector (Fin BB) 50)
       refine congr_arg (BitVec.ofNat 64) ?_
       simp [BitVec.toNat_ofNat]
       omega
-    · apply congr_arg₂ s.mem.insert
-      · simp [Word.toBitVec64, Word.toNat, sp1_imm_c,
-          BitVec.ofNat_add]
-        congr 4
-        simp [BitVec.toNat_eq]
-        omega
-      · simp [BitVec.toNat_eq]
+    have h1221 : (BitVec.ofNat 12 (Word.toNat #v[Main[21], Main[22], Main[23], Main[24]])) =
+      BitVec.ofNat 12 Main[21] := by simp [Word.toNat, BitVec.ofNat_add, BitVec.ofNat_mul]
+    simp [h1221]
 
   -- Other hypothesis for the lemma
   · simp [SailState.isInitialized, hs]
   · simpa using h14_op_a
   · simp [is_aligned_vaddr]
+    sorry
   · constructor <;> simpa [Std.ExtDHashMap.get_insert]
   · simpa [Std.ExtDHashMap.get_insert]
 
