SP1Chips.lean
@@ -38,6 +38,9 @@ import SP1Chips.Store.StoreDouble.Constraints
 import SP1Chips.Store.StoreHalf.Constraints
 import SP1Chips.Store.StoreWord.Constraints
 import SP1Chips.StoreByteChip
+import SP1Chips.StoreDoubleChip
+import SP1Chips.StoreHalfChip
+import SP1Chips.StoreWordChip
 import SP1Chips.Sub.Constraints
 import SP1Chips.SubChip
 import SP1Chips.Subw.Constraints
