SP1Foundations/MemChecks.lean
@@ -9,14 +9,15 @@ axiom pmp_check_machine (reg_val : BitVec 64) (offset : BitVec 64)
 
 /-- For good states there is no `mmio` region. -/
 lemma run_within_mmio_writable_mmio (reg_val : BitVec 64) (offset : BitVec 64)
-    (s : SailState) (hs : SailState.isInitialized s)
+    (width : ℕ) (hw : 0 < width) (s : SailState) (hs : SailState.isInitialized s)
     (hclint_base : s.regs.get Register.plat_clint_base (hs _) = 0)
     (hclint_size : s.regs.get Register.plat_clint_size (hs _) = 0) :
     (within_mmio_writable (physaddr.Physaddr
-      (zero_extend (BitVec.addInt (reg_val + offset) 0))) 1).run s = .ok false s := by
+      (zero_extend (BitVec.addInt (reg_val + offset) 0))) width).run s = .ok false s := by
   simp [within_mmio_writable, get_config_rvfi, within_clint]
   simp [run_readReg_of_isInitialized s _ hs, hclint_base, hclint_size]
   simp [within_htif_writable, htif_tohost_base]
+  omega
 
 /-- For good states there is not `phys_mem` bound on size. -/
 lemma run_within_phys_mem (reg_val : BitVec 64) (offset : BitVec 64)
